\documentclass[10pt,fleqn]{article}
\newcommand{\name}[1]{\def\psettitlename{#1}}
\newcommand{\course}[1]{\def\psettitlecourse{#1}}
\newcommand{\rsection}[1]{\def\psettitlersection{#1}}
\newcommand{\psetnum}[1]{\def\psettitlepsetnum{#1}}
%\usepackage[journal=rsc]{chemstyle}
%\usepackage{mhchem}
\usepackage{amsmath}
\usepackage{amssymb}
\usepackage{amsfonts}
\usepackage{esint}
\usepackage{bbm}
\usepackage{amscd}
\usepackage{picinpar}
\usepackage[pdftex]{graphicx}
\usepackage{tikz}
\usepackage{indentfirst}
\usepackage{wrapfig}
\usepackage{units}
\usepackage{textcomp}
\usepackage[utf8x]{inputenc}
% \usepackage{feyn}
\usepackage{feynmp}
\usetikzlibrary{
  arrows,
  calc,
  decorations.pathmorphing,
  decorations.pathreplacing,
  decorations.markings,
  fadings,
  positioning,
  shapes
}

\DeclareGraphicsRule{*}{mps}{*}{}
\newcommand{\ud}{\mathrm{d}}
\newcommand{\ue}{\mathrm{e}}
\newcommand{\ui}{\mathrm{i}}
\newcommand{\res}{\mathrm{Res}}
\newcommand{\Tr}{\mathrm{Tr}}
\newcommand{\dsum}{\displaystyle\sum}
\newcommand{\dprod}{\displaystyle\prod}
\newcommand{\dlim}{\displaystyle\lim}
\newcommand{\dint}{\displaystyle\int}
\newcommand{\fsno}[1]{{\!\not\!{#1}}}
\newcommand{\eqar}[1]
{
  \begin{align*}
    #1
  \end{align*}
}
\newcommand{\texp}[2]{\ensuremath{{#1}\times10^{#2}}}
\newcommand{\dexp}[2]{\ensuremath{{#1}\cdot10^{#2}}}
\newcommand{\eval}[2]{{\left.{#1}\right|_{#2}}}
\newcommand{\paren}[1]{{\left({#1}\right)}}
\newcommand{\lparen}[1]{{\left({#1}\right.}}
\newcommand{\rparen}[1]{{\left.{#1}\right)}}
\newcommand{\abs}[1]{{\left|{#1}\right|}}
\newcommand{\sqr}[1]{{\left[{#1}\right]}}
\newcommand{\crly}[1]{{\left\{{#1}\right\}}}
\newcommand{\angl}[1]{{\left\langle{#1}\right\rangle}}
\newcommand{\tpdiff}[4][{}]{{\paren{\frac{\partial^{#1} {#2}}{\partial {#3}{}^{#1}}}_{#4}}}
\newcommand{\tpsdiff}[4][{}]{{\paren{\frac{\partial^{#1}}{\partial {#3}{}^{#1}}{#2}}_{#4}}}
\newcommand{\pdiff}[3][{}]{{\frac{\partial^{#1} {#2}}{\partial {#3}{}^{#1}}}}
\newcommand{\diff}[3][{}]{{\frac{\ud^{#1} {#2}}{\ud {#3}{}^{#1}}}}
\newcommand{\psdiff}[3][{}]{{\frac{\partial^{#1}}{\partial {#3}{}^{#1}} {#2}}}
\newcommand{\sdiff}[3][{}]{{\frac{\ud^{#1}}{\ud {#3}{}^{#1}} {#2}}}
\newcommand{\tpddiff}[4][{}]{{\left(\dfrac{\partial^{#1} {#2}}{\partial {#3}{}^{#1}}\right)_{#4}}}
\newcommand{\tpsddiff}[4][{}]{{\paren{\dfrac{\partial^{#1}}{\partial {#3}{}^{#1}}{#2}}_{#4}}}
\newcommand{\pddiff}[3][{}]{{\dfrac{\partial^{#1} {#2}}{\partial {#3}{}^{#1}}}}
\newcommand{\ddiff}[3][{}]{{\dfrac{\ud^{#1} {#2}}{\ud {#3}{}^{#1}}}}
\newcommand{\psddiff}[3][{}]{{\frac{\partial^{#1}}{\partial{}^{#1} {#3}} {#2}}}
\newcommand{\sddiff}[3][{}]{{\frac{\ud^{#1}}{\ud {#3}{}^{#1}} {#2}}}
\usepackage{fancyhdr}
\usepackage{multirow}
\usepackage{fontenc}
%\usepackage{tipa}
\usepackage{ulem}
\usepackage{color}
\usepackage{cancel}
\newcommand{\hcancel}[2][black]{\setbox0=\hbox{#2}%
\rlap{\raisebox{.45\ht0}{\textcolor{#1}{\rule{\wd0}{1pt}}}}#2}
\pagestyle{fancy}
\setlength{\headheight}{67pt}
\fancyhead{}
\fancyfoot{}
\fancyfoot[C]{\thepage}
\fancyhead[R]
{
\psettitlename \\
\psettitlecourse{} Problem Set \psettitlepsetnum \\
\ifx\psettitlersection\empty
\else
Recitation Section \psettitlersection
\fi
}
\renewcommand{\footruleskip}{0pt}
\renewcommand{\headrulewidth}{0.4pt}
\renewcommand{\footrulewidth}{0pt}
\addtolength{\hoffset}{-1.3cm}
\addtolength{\voffset}{-2cm}
\addtolength{\textwidth}{3cm}
\addtolength{\textheight}{2.5cm}
\renewcommand{\footskip}{10pt}
\setlength{\headwidth}{\textwidth}
\setlength{\headsep}{20pt}
\setlength{\marginparwidth}{0pt}
\parindent=0pt
\psetnum{2}
\input{../head}
\begin{document}
\section{}
\subsection{}
\eqar{
  x_i'x_i'=&a_{ij}a_{ik}x_jx_k\\
  x_ix_i=&\delta_{jk}x_jx_k
  \intertext{Since $x_i'x_i'=x_ix_i$ for all $x_i$}
  \delta_{jk}=&a_{ij}a_{ik}
}
\subsection{}
\eqar{
  x_i=&\delta_{ik}x_k\\
  =&a_{ji}a_{jk}x_k\\
  =&a_{ji}x_j'
}
\subsection{}
\eqar{
  \pdiff{f}{x_i'}=&\pdiff{f}{x_j}\pdiff{x_j}{x_i'}\\
  =&\pdiff{f}{x_j}\pdiff{a_{kj}x_k'}{x_i'}\\
  =&a_{ij}\pdiff{f}{x_j}
}

\section{}
\subsection{}
\eqar{
  \delta_{ij}'=&a_{im}a_{jn}\delta_{mn}\\
  =&a_{ik}a_{jk}\\
  =&\delta_{ij}
}
\subsection{}
\eqar{
  C'_iT'_{ij}=&a_{ik}C_ka_{im}a_{jn}T_{mn}\\
  =&a_{ik}a_{im}a_{jn}C_kT_{mn}\\
  =&\delta_{km}a_{jn}C_kT_{mn}\\
  =&a_{jk}C_iT_{ik}\\
  =&(C_iT_{ik})'
}
\subsection{}
Since both $A_iA_j$ and $\delta_{ij}$ are second rank tensors and $A^2$ is a scalar, $T_{ij}$ is also a second rank tensor.
\subsection{}
\eqar{
  &\partial_i\paren{A_iA_j-\frac12\delta_{ij}A_kA_k}\\
  =&\partial_i\paren{A_iA_j}-\frac12\partial_j\paren{A_kA_k}\\
  =&A_j\partial_i\paren{A_i}+A_i\partial_i\paren{A_j}-A_k\partial_j\paren{A_k}\\
  =&A_j\partial_i\paren{A_i}+A_i\partial_i\paren{A_j}-A_i\partial_j\paren{A_i}\\
  =&A_j\partial_i\paren{A_i}+A_i\paren{\delta_{ki}\delta_{jl}-\delta_{jk}\delta{il}}\partial_k\paren{A_l}\\
  =&A_j\partial_i\paren{A_i}+\varepsilon_{mij}A_i\varepsilon_{mkl}\partial_k\paren{A_l}\\
  =&A_j\partial_i\paren{A_i}+\varepsilon_{jmi}\paren{\varepsilon_{mkl}\partial_k\paren{A_l}}A_i
}
\subsection{}
\subsubsection{}
\eqar{
  T_{ij}n_j=&\paren{A_iA_j-\frac12\delta_{ij}A^2}n_j\\
  =&A_iA_jn_j-\frac12A^2n_i
}
Therefore $T\cdot\vec n$ is a linear combination of $\vec A$ and $\vec n$
\subsubsection{}
Let $B_i=T_{ij}n_j$
\eqar{
  B_iB_i=&\paren{A_iA_jn_j-\frac12A^2n_i}\paren{A_iA_kn_k-\frac12A^2n_i}\\
  =&\paren{A_jn_j}^2A^2+\frac14A^4-\paren{A_jn_j}^2A^2
  =&\frac14A^4\\
  B_in_i=&A_iA_jn_jn_i-\frac12A^2\\
  =&A^2\paren{\cos^2\theta-\frac12}\\
  =&\frac{A^2}2\cos2\theta\\
  \cos\theta_{Bn}=&\cos2\theta\\
  \theta_{Bn}=&2\theta
}
\subsubsection{}
See above.

\section{}
\subsection{}
\eqar{
  E_r=&\frac{\lambda}{2\pi\varepsilon_0 r}-E_0\sin\phi\\
  E_\phi=&-E_0\cos\phi
}
\subsection{}
\eqar{
  E_r=&\frac{2\pi\varepsilon_0 E_0\lambda}{2\pi\varepsilon_0 \lambda}-E_0\\
  =&0\\
  E_\phi=&0
}
\subsection{}
\eqar{
  \ud\vec F=&\varepsilon_0r\ud\phi\ud z\paren{E_r\vec E-\frac{1}{2}E^2\hat r}\\
  =&\varepsilon_0r\ud\phi\ud z\paren{\frac{E_r^2-E_\phi^2}2\hat r+E_rE_\phi\hat\phi}
}
\subsection{}
\eqar{
  \diff{\vec F}{z}=&\int\varepsilon_0r\ud\phi\paren{\frac{E_r^2-E_\phi^2}2\hat r+E_rE_\phi\hat\phi}\\
  =&\frac{\varepsilon_0r}2\hat y\int\ud\phi\paren{\paren{\paren{\frac{\lambda}{2\pi\varepsilon_0 r}-E_0\sin\phi}^2-E_0\cos^2\phi}\sin\phi-2\paren{\frac{\lambda}{2\pi\varepsilon_0 r}-E_0\sin\phi}E_0\cos^2\phi}\\
  =&\frac{\varepsilon_0r}2\hat y\int\ud\phi\paren{-2\frac{\lambda}{2\pi\varepsilon_0 r}E_0\sin^2\phi-\frac{\lambda}{\pi\varepsilon_0 r}E_0\cos^2\phi}\\
  =&\frac{1}2\hat y\int\ud\phi\paren{-\frac{\lambda}{\pi}E_0\sin^2\phi-\frac{\lambda}{\pi}E_0\cos^2\phi}\\
  =&-\frac{1}2\hat y2\pi\frac{\lambda}{\pi}E_0\\
  =&-E_0\lambda\hat y
}

\section{}
\subsection{}
\eqar{
  B_r=&B_0\sin\phi\\
  B_\phi=&\frac{\mu_0 I}{2\pi r}+B_0\cos\phi
}
\subsection{}
\eqar{
  B_r=&0\\
  B_\phi=&\frac{\mu_0 I2\pi B_0}{2\pi \mu_0I}+B_0\\
  =&0
}
\subsection{}
\eqar{
  \ud\vec F=&\frac1\mu_0r\ud\phi\ud z\paren{B_r\vec B-\frac{1}{2}B^2\hat r}\\
  =&\frac1\mu_0r\ud\phi\ud z\paren{\frac{B_r^2-B_\phi^2}2\hat r+B_rB_\phi\hat\phi}
}
\subsection{}
\eqar{
  \diff{\vec F}{z}=&\frac12\int\frac{r}{\mu_0}\ud\phi\paren{\paren{B_r^2-B_\phi^2}\hat r+2B_rB_\phi\hat\phi}\\
  =&\frac{r\hat x}{2\mu_0}\int\ud\phi\paren{\paren{B_0^2\sin^2\phi-\paren{\frac{\mu_0 I}{2\pi r}+B_0\cos\phi}^2}\cos\phi-2B_0\sin\phi\paren{\frac{\mu_0 I}{2\pi r}+B_0\cos\phi}\sin\phi}\\
  =&\frac{r\hat x}{2\mu_0}\int\ud\phi\paren{-\paren{\frac{\mu_0 I}{2\pi r}+B_0\cos\phi}^2\cos\phi-B_0\sin^2\phi\frac{\mu_0 I}{\pi r}}\\
  =&\frac{\hat x}{2}\int\ud\phi\paren{-\frac{I}{\pi}B_0\cos^2\phi-B_0\sin^2\phi\frac{I}{\pi}}\\
  =&-B_0I\hat x\\
}

\section{}
\subsection{}
\eqar{
  \vec E_{line}=&\frac{\lambda\paren{\vec r-\vec Y}}{2\pi\varepsilon_0\paren{\vec r-\vec Y}^2}\\
  =&\frac{\lambda\paren{x\hat x+\paren{y-Y}\hat y}}{2\pi\varepsilon_0\paren{x^2+\paren{y-Y}^2}}\\
  E=&\frac{\lambda\paren{x\hat x+\paren{y-Y}\hat y}}{2\pi\varepsilon_0\paren{x^2+\paren{y-Y}^2}}-E_0\hat y
}
\subsection{}
\eqar{
  &\int_{-\infty}^\infty\ud x\int_{-L}^L\ud y\varepsilon_0\vec E_0\cdot\vec E_{line}\\
  =&-\int_{-\infty}^\infty\ud x\int_{-L}^L\ud y\varepsilon_0\frac{\lambda\paren{x\hat x+\paren{y-Y}\hat y}}{2\pi\varepsilon_0\paren{x^2+\paren{y-Y}^2}}E_0\cdot\hat y\\
  =&-\frac{E_0\lambda}{2\pi}\int_{-\infty}^\infty\ud x\int_{-L}^L\ud y\frac{y-Y}{x^2+\paren{y-Y}^2}\\
  =&-\frac{E_0\lambda}{4\pi}\int_{-\infty}^\infty\ud x\ln\paren{\frac{x^2+\paren{L-Y}^2}{x^2+\paren{-L-Y}^2}}
  \intertext{Let $\alpha=\dfrac xL$, $\beta=\dfrac YL$}
  \diff{E}{z}=&-\frac{E_0\lambda}{4\pi}\int_{-\infty}^\infty\ud\alpha\ln\paren{\frac{\alpha^2+\paren{1-\beta}^2}{\alpha^2+\paren{1+\beta}^2}}\\
  =&-\frac{E_0\lambda}{4\pi}\int_{-\infty}^\infty\ud\alpha\ln\paren{\frac{\alpha^2+1-2\beta}{\alpha^2+1+2\beta}}\\
  \approx&-\frac{E_0\lambda L}{4\pi}\int_{-\infty}^\infty\ud\alpha\frac{4\beta}{1+\alpha^2}\\
  =&-E_0\lambda Y
}

\end{document}
